Ownership.dfy
@@ -1,6 +1,6 @@
 include "Library.dfy"
 include "Object.dfy"
-
+include "Bound.dfy"
 
 //[[[[[[[[[[[[[[[[[[[[[[[[[[[[[[[[[[[[[[[[]]]]]]]]]]]]]]]]]]]]]]]]]]]]]]]]]]]]]]]]
 //[[[[[[[[[[[[[[[[[[[[[[[[[[[[[[[[[[[[[[[[]]]]]]]]]]]]]]]]]]]]]]]]]]]]]]]]]]]]]]]]
@@ -192,7 +192,8 @@ predicate nuBoundsOK(oo : Owner, mb : Owner) {
 //arguments are local fields, unflattened...
 //&& (flatten(mb) <= flatten(oo))  //bound is a subset of owner
   && (flatten(oo) >= flatten(mb)) //aka effectiveowner is INSIDE effectivebound
-//  && (forall o <- oo :: o.AMFB >= flatten(mb))
+
+  && (forall o <- oo :: o.AMFB >= flatten(mb))
 
 //  && (flatten(mb) <= (set ooo <- oo, omb <- ooo.AMFB :: omb) + oo)
       //AKA (I think) effectivebound is subseteq/surroundingeq the union of owners' bounds.
