Xlone-Seed.dfy
@@ -1,6 +1,7 @@
 include "Klon.dfy"
 include "Context.dfy"
 include "Xlone.dfy"
+include "Bound.dfy"
 
 method {:isolate_assertions} clone(a : Object, context : set<Object>,  into : Owner := a.owner)
     returns (b : Object, subtext : set<Object>)
@@ -8,94 +9,95 @@ decreases *
   requires COK(a, context)
   requires flatten(into) >= a.AMFB
   requires CallOK(context)
+    requires context >= flatten(into) >= flatten(into)   //GRR
+    requires flatten(into) >= flatten(into)
+    requires forall o <- flatten(into) :: o.Ready()
+    requires myBoundsOK(into, into)  //hmm
   requires forall x <- context :: x.Ready() && x.AllOutgoingReferencesWithinThisHeap(context)
 {
   var m0 : Klon := seed(a, into, context);
+
+  assert m0.StupidCalidFragilistic();
+
   var m1 : Klon;
 
-  assume m0.SuperCalidFragilistic();  ///HMMMM.
+  reveal COK();
+
   assert COK(a, m0.oHeap);
   assert klonCanKV(m0,a,a);
 
-  b, m1 := Xlone_Via_Map(a, m0);
 
-  subtext := m1.hns();
+  b := new Object.make(a.fieldModes, m0.clowner, m0.oHeap, "clone_of_" + a.nick, m0.clbound);
+
+    assert m0.StupidCalidFragilistic();
+    assert a.Ready();
+    assert m0.ownersInKlown(a);
+    assert m0.o.Ready();
+    assert m0.objectInKlown(m0.o);
+    assert m0.CalidCanKey(a);
+    assert a !in m0.m.Keys;
+    assert b !in m0.m.Values;
+    assert a in m0.oHeap;
+    assert b.Ready() ;
+    assert b.Valid() ;
+    assert b.Context(m0.hns({b}));
+    assert m0.m.Keys <= m0.oHeap;
+    assert klonVMapOK(m0.m);
+    assert klonCanKV(m0,a,b);
+    assert m0.CalidLineKV(a,b);
+
+  assert m0.CKV_preconditions(a,b);
+  assert m0.CalidLineKV(a,b);
+
+  assert m0.StupidCalidFragilistic();
+  assert m0.ownersInKlown(m0.o);
+
+  m1 := m0.CalidKV(a,b);
+  assert a == m0.o == m1.o;
+  assert m1.o in m1.m.Keys;
+  assert m1.objectInKlown(m1.o);
+  assert m1.SuperCalidFragilistic();
+  var rm := Xlone_All_Fields(a,b,m1);
+  assert rm.SuperCalidFragilistic();
+  subtext := rm.hns();
 }
 
-//   var m' : Klon := Klon(map[],    //m clonemap
-//                a,       // o - object to be cloned / pivot / top object
-//                a.AMFO,  // o_amfo AMFO of o
-//                into,    // c_owner - proposewd owner of clone
-//                flatten(into),   // c_amfx - AMFX of clone
-//                {},
-//                {},
-//                context,      // oHeap
-//                {}            // ns );
-//               );
-//
-//   assert a in context;
-//   assert m'.m.Keys == {} == m'.m.Values;
-//
-//   assert m'.calid() by {
-//
-//     reveal m'.calidObjects(); assert m'.calidObjects();
-//     reveal m'.calidOK();
-//
-//     assert (m'.o in m'.oHeap);
-//     assert (m'.m.Keys <= m'.oHeap);
-//     assert (m'.m.Values <= m'.oHeap+m'.ns);
-//     assert COK(m'.o, m'.oHeap);
-//     assert CallOK(m'.oHeap);
-//
-//     reveal CallOK();
-//     assert CallOK(m'.m.Keys, m'.oHeap) by { assert m'.m.Keys == {}; }
-//     assert CallOK(m'.m.Values, m'.oHeap+m'.ns) by { assert m'.m.Values == {}; }
-//     assert CallOK(m'.ns, m'.oHeap+m'.ns) by { assert m'.ns == {}; }
-//
-//     assert forall x <- m'.oHeap :: x.Ready() && x.AllOutgoingReferencesWithinThisHeap(m'.oHeap);
-//
-//
-//     assert m'.calidOK();
-//     reveal m'.calidMap();     assert m'.calidMap();
-//     reveal m'.calidSheep();   assert m'.calidSheep();
-//
-//     reveal m'.calid();        assert m'.calid();
-//   }
-//
-//
-//   assert allMapOwnersThruKlownOK(m');
-//
-//   assert klonCanKV(m',a,a);
-//
-// //  assert m'.readyAll() by { assert m'.m.Keys == {}; }
-//
-//   assert forall o <- m'.m.Keys :: mappingOwnersThruKlownOK(o,m');
-//
-//   assert allMapOwnersThruKlownOK(m');
-//
-//   assert klonCanKV(m',a,a);  //hmm, interesting... technically not right but;
-//         //not, this IS ruight...
+lemma {:isolate_assertions} STOOPID(x : Object, oHeap : set<Object>)
+   requires COK(x,oHeap)
+    ensures reveal COK(x); COK(x,oHeap) && x.Ready() && x.Valid() && x.Context(oHeap)
+  {
+  assert COK(x,oHeap);
+  reveal COK();
+  assert x.Ready() && x.Valid() && x.Context(oHeap);
+  }
 
+lemma {:isolate_assertions} STOOPID_TOO(m : Klon)
+   requires m.StupidCalidFragilistic()
+   requires m.objectInKlown(m.o)
+    ensures m.SuperCalidFragilistic()
+{}
 
-
-function {:isolate_assertions} {:timeLimit 30}  seed(o : Object, clowner : Owner, oHeap : set<Object>) : (m : Klon)
+function {:isolate_assertions} {:timeLimit 15}  seed(o : Object, clowner : Owner, oHeap : set<Object>) : (m : Klon)
 //seed Klon for cloning object o,  owner of clone being clowner, within heap oHeap...
     requires COK(o, oHeap)
     requires CallOK(oHeap)
     requires forall x <- oHeap :: x.Ready() && x.AllOutgoingReferencesWithinThisHeap(oHeap)
-//    ensures m.apoCalidse()
+
+    requires oHeap >= flatten(clowner) >= flatten(clowner)   //GRR
+    requires flatten(clowner) >= flatten(clowner)
+    requires forall o <- flatten(clowner) :: o.Ready()
+    requires myBoundsOK(clowner, clowner)
+    requires myBoundsOK(o.owner, o.bound)  //GRR update ready?
 
     ensures (m.m.Keys <= m.oHeap)
     ensures (m.m.Values <= m.hns())
     ensures (m.ownersReadyInKlown(o))  //not obejctReadyInCloneapparentlyt...  FUCK need to look at Xlone-MAIN I BET
     ensures (m.HeapOwnersReady())
     ensures (m.c_amfx <= m.oHeap)
+    ensures forall x <- oHeap :: (x.Ready() && x.Valid() && x.Context(oHeap))
 
-//    ensures m.ownersInKlow n(o)
-//    ensures m.SuperCalidFragilistic()
-//    ensures COK(o, m.oHeap)
-
-
+    ensures m.StupidCalidFragilistic() /// cos obkject aint in the KLON at this ponmt..
+    ensures COK(o, m.oHeap)
 //    ensures allMapOwnersThruKlownIfInsideOK(m)
 //
 //     ensures m == Klon( (map x <- o.AMFX :: x),
@@ -108,9 +110,12 @@ function {:isolate_assertions} {:timeLimit 30}  seed(o : Object, clowner : Owner
 //         oHeap,
 //         {} )
 
-
     reads oHeap`fields, oHeap`fieldModes
     {
+     assert CallOK(oHeap); reveal CallOK(); reveal COK();
+     assert forall x <- oHeap :: (reveal COK(); COK(x,oHeap));
+     assert forall x <- oHeap :: (reveal COK(); COK(x,oHeap) && x.Ready() && x.Valid() && x.Context(oHeap));
+     assert forall x <- oHeap :: (x.Ready() && x.Valid() && x.Context(oHeap));
 
     var mep0 := map x <- o.AMFX :: x;
 
@@ -124,9 +129,13 @@ function {:isolate_assertions} {:timeLimit 30}  seed(o : Object, clowner : Owner
 
     assert mep.Keys == mep.Values == o.AMFX <= oHeap by  { reveal COK(); }
 
-    forall x <- mep0.Keys ensures true //by
+    forall x <- mep.Keys ensures true //by
       {
         assert x.Ready();
+        assert outside(x,o);
+        assert (inside(x,o)) ==> (mep[x] !in oHeap);
+        assert x in oHeap;
+
         //assert mep0.Keys >= o.AMFX >= o.AMFB;
         //assert mep0.Keys >= mep0[o].AMFX >= mep0[o].AMFB;
       }
@@ -136,18 +145,63 @@ function {:isolate_assertions} {:timeLimit 30}  seed(o : Object, clowner : Owner
 
 
 
-    var m : Klon :=
-                       Klon(mep,
+    var m : Klon := Klon(mep,
                             o,
 //                          o.AMFX,
                             clowner,
-                            clowner,
+                            proposeBounds(clowner),
                             // clamfx,
                             // oxtra,
                             // cxtra,
                             oHeap,
                             o.AMFX,
                             clamfx);
+
+// assert forall x <- m.m.Keys :: (
+//     && (outside(x,m.o))
+//     && (x.AMFX <= m.m.Keys)
+//     && (x.AMFB <= m.m.Keys)
+// //    && (k.bound <= k.owner <= m.Keys)
+//     && (m.ownersInKlown(x))  //belt and braces--- currently a requirement!
+//
+//   && (x.Ready())
+//   && (m.ownersInKlown(x))
+//   && (x.Ready())
+//   && (m.apoCalidse())
+//   && (x.owner <= m.m.Keys <= m.oHeap)
+//   && (m.m.Values <= flatten( m.hns() ))
+//   && (m.o.Ready())
+//   && (m.HeapOwnersReady())
+//   && (m.c_amfx <= m.oHeap)
+//
+//     && (checkOwnershipOfClone(x,x,m))
+//     && (checkBoundOfClone(x,x,m))
+//     && (mappingOwnersThruKlownKV(x,x,m))
+// );
+
+
+forall x <- m.m.Keys ensures (true) //GRRR (m.CalidLineKV(x,x)) //by
+{
+    assert (outside(x,m.o));
+    assert (x.AMFX <= m.m.Keys);
+    assert (x.AMFB <= m.m.Keys);
+    assert (m.ownersInKlown(x)) ;
+    assert (x.Ready());
+    assert (m.ownersInKlown(x));
+    assert (x.Ready());
+//    assert (m.apoCalidse());
+    assert (x.owner <= m.m.Keys <= m.oHeap);
+    assert (m.m.Values <= flatten( m.hns() ));
+    assert (m.o.Ready());
+    assert (m.HeapOwnersReady());
+    assert (m.c_amfx <= m.oHeap);
+    assert (checkOwnershipOfClone(x,x,m));
+    assert (checkBoundOfClone(x,x,m));
+    assert (mappingOwnersThruKlownKV(x,x,m));
+}
+
+// assert forall x <- m.m.Keys :: m.CalidLineKV(x,x);
+
 
   // assert m.hns() == oHeap + clamfx;
     assert m.oHeap == oHeap;
@@ -162,15 +216,15 @@ function {:isolate_assertions} {:timeLimit 30}  seed(o : Object, clowner : Owner
     assert CallOK(oHeap);
     assert forall x <- oHeap :: x.Ready();
 
-assert m.o.Ready();
-assert (m.o.AMFX <= m.m.Keys);
+    assert m.o.Ready();
+    assert (m.o.AMFX <= m.m.Keys);
 
 
-//     assert (m.m.Keys <= m.oHeap);
-//     assert (m.m.Values <= m.hns());
-//    assert (m.objectReadyInKlown(o));
-//     assert (m.HeapOwnersReady());
-//     assert (m.c_amfx <= m.oHeap);
+    assert (m.m.Keys <= m.oHeap);
+    assert (m.m.Values <= m.hns());
+    assert (m.ownersReadyInKlown(o));
+    assert (m.HeapOwnersReady());
+    assert (m.c_amfx <= m.oHeap);
 
     m
     }
